

Tutorial - 1

Name :- Gaurang Seemastawa
Section :- F
Roll No :- 57
Univ. Roll No :- 2016746.

Q.1. What

Ans 1. Asymptotic Notation are the mathematical notations used to describe the running time of an algorithm.

Different types of Asymptotic Notation :-

1) Big O Notation (O) :- It represents upper bound of algorithm.

$$f(n) = O(g(n)) \text{ if } f(n) \leq c * g(n)$$

2) Omega Notation (Ω) :- It represents lower bound of algorithm

$$f(n) = \Omega(g(n)) \text{ if } f(n) \geq c * g(n)$$

3) Theta Notation (Θ) :- It represents upper and lower bound of algorithm

$$f(n) = \Theta(g(n)) \text{ if } c_1 g(n) \leq f(n) \leq c_2 g(n).$$

Ans 2. for ($i = 1$ to n).

~~do~~ {
 $i = i * 2$;
}

$i = 1$
 $i = 2$
 $i = 4$
 $i = 8$
 $i = 16$
 $i = n$

It is forming n^P .

$$\begin{aligned} a_n &= a_{n-1} \\ n &= a_{n-1}^{K-1} \\ n &= 1 \times (2)^{K-1} \end{aligned}$$

$$\left(\begin{array}{l} a_n = n \\ n = 2 \\ a = 1 \end{array} \right)$$

$$\begin{aligned} \log n &= \log 2^{K-1} \\ \log n &= (K-1) \log 2. \end{aligned}$$

$$K = \log n + 1.$$

$$O(\log n)$$

Ans 3

$$T(n) = 3T(n-1) \quad \text{if } n > 0, \text{ otherwise } 1$$

$$T(1) = 3T(0). \quad [T(0) = 1]$$

$$T(1) = 3 \times 1$$

$$T(2) = 3T(1) = 3 \times 3 \times 1$$

$$T(3) = 3 \times T(2) = 3 \times 3 \times 3$$

⋮

$$T(n) = 3 \times 3 \times 3 \dots$$

$$= 3^n = O(3^n)$$

Ans 4

$$T(n) = 2T(n-1) - 1 \quad \text{if } n > 0, \text{ otherwise } 1$$

$$T(0) = 1$$

$$T(1) = 2T(0) - 1$$

$$T(1) = 2 - 1 = 1$$

$$T(2) = 2T(1) - 1$$

$$T(2) = 2 - 1 = 1$$

$$T(3) = 2T(2) - 1$$

$$= 2 - 1 = 1$$

⋮

$$T(n) = 1 \quad O(1)$$

Ans 5

int i = 1, j = 1

while (i ≤ n).

{

i++;

j = j + i;

printf("%d\n", j);

}

③

$i = 1$ $S = 1$
 $i = 2$ $S = 1 + 2$
 $i = 3$ $S = 1 + 2 + 3$
 $i = 4$ $S = 1 + 2 + 3 + 4$
⋮

loop ends when

$$\begin{aligned} S &> n \\ 1 + 2 + 3 + 4 + \dots + K &> n \\ \frac{K(K+1)}{2} &> n \\ K^2 &> n \\ K &> \sqrt{n} \\ &= O(\sqrt{n}) \end{aligned}$$

Ans 6 void function (int n)

```
{  
    int i, count = 0;  
    for (int i = 1; i * i <= n; i++)  
        count++;  
}
```

loop ends when $i * i > n$

$$\begin{aligned} K * K &> n \\ K^2 &> n \\ K &> \sqrt{n} \\ O(n) &= \sqrt{n} \end{aligned}$$

$i = 1$
 $i = 2$
 $i = 3$
 $i = 4$
⋮
 $i = K$

Ans 7 Void function (int n).

```

{
    int i, j, k, count = 0;
    for (i = n/2; i <= n; i++)
    {
        for (j = 1; j <= n; j = j * 2)
            for (k = 1; k <= n; k = k * 2)
                count++;
    }
}

```

• 1st loop: $i = \frac{n}{2}$ to n , $i++$.
 $= O(\frac{n}{2}) = O(n)$.

• 2nd Nested Loop: $j = 1$ to n ; $j = j * 2$
 $j = 1$
 $j = 2$
 $j = 4$
 $j = n$
 $= O(\log n)$.

• 3rd Nested Loop: $k = 1$ to n , $k = k * 2$.
 $k = 1$
 $k = 2$
 $k = 4$
 $= O(\log n)$.

Total complexity = $O(n \times \log n \times \log n) = O(n \log^2 n)$.

Ans 8 Function (int n)

```

{
    if (n == 1) return; — 1
    for (int i = 1 to n)
    {
        for (int j = 1 to n) —  $n^2$ 
        {
            printf("*");
        }
    }
    function (n-3) —  $T(n-3)$ 
}

```

Highway merge...

(5)

$$T(n) = T(n-3) + n^2$$

$$\rightarrow T(1) = 1$$

$$T(4) = T(4-3) + 4^2$$

$$= T(1) + 4^2 = 1^2 + 4^2$$

$$T(7) = T(7-3) + 7^2$$

$$= 1^2 + 4^2 + 7^2$$

$$T(10) = T(10-3) + 10^2$$

$$= 1^2 + 4^2 + 7^2 + 10^2$$

$$\text{So, } T(n) = 1^2 + 4^2 + 7^2 + 10^2 + \dots + n^2 = \frac{n(n+1)(2n+1)}{6} = O(n^3)$$

also for terms like $T(2), T(3), T(5)$.

$$\text{So, } T(n) = O(n^3)$$

Ans 9

Void function (int n).

{

for (int i = 1 to n) — n.

{ for (j = 1; j <= n; j = j + 1) — n.

{ printf ("%*");

}

}

}

i = 1 — j = 1 to n.

i = 2 — j = 1 to n

i = 3 — j = 1 to n

i = 4 — j = 1 to n.

So, for i upto n it will take

$$n^2$$

$$\text{So, } T(n) = O(n^2).$$

Ans 10:

$$f_1(n) = n^K$$

$$, f_2(n) = c^n.$$

Asymptotic relationship b/w f_1 & f_2 .

$$K \geq 1, c > 1$$

$$\text{is Big O i.e. } f_1(n) = O(f_2(n)) = O(c^n).$$

$$\text{in } n^K \leq G * c^n \quad [G \text{ is some constant}]$$